feat: tactics chapter (#34)

Main.lean
@@ -6,13 +6,12 @@ open Verso.Genre.Manual
 
 
 def main :=
-  manualMain (%doc Manual)
-    (config := config)
+  manualMain (%doc Manual) (config := config)
 where
   config := {
     extraFiles := [("static", "static")],
-    extraCss := ["/static/colors.css", "/static/theme.css", "/static/inter/inter.css", "/static/firacode/fira_code.css", "/static/katex/katex.min.css"],
-    extraJs := ["/static/katex/katex.min.js", "/static/math.js"]
+    extraCss := ["/static/colors.css", "/static/theme.css", "/static/print.css", "/static/inter/inter.css", "/static/firacode/fira_code.css", "/static/katex/katex.min.css"],
+    extraJs := ["/static/katex/katex.min.js", "/static/math.js", "/static/print.js"]
     emitTeX := false
-    emitHtmlSingle := false
+    emitHtmlSingle := true -- for proofreading
   }
