Manual.lean
@@ -3,6 +3,9 @@ import VersoManual
 import Manual.Intro
 import Manual.Elaboration
 import Manual.Language
+import Manual.Terms
+import Manual.Tactics
+import Manual.Simp
 import Manual.BuiltInTypes
 
 open Verso.Genre Manual
@@ -21,14 +24,42 @@ authors := ["Lean Developers"]
 
 {include Manual.Language}
 
-{include Manual.BuiltInTypes}
+{include Manual.Terms}
+
+# Monads and `do`-Notation
+
+# IO
+
+{include 0 Manual.Tactics}
+
+{include 0 Manual.Simp}
+
+{include 0 Manual.BuiltInTypes}
+
+# Notations and Macros
+
+:::planned
+A presentation of macros, covering
+ * `notation`
+ * Definition of {deftech}_macro_
+ * Syntax extension and syntax categories
+   * Precedence
+ * `macro_rules`
+   * Syntax patterns
+   * Backtracking on expansion failure
+ * {deftech}[Hygiene] and quotation
+ * The `macro` command
+:::
+
+# Lake and Reservoir
+
 
 
 # Progress
 
 :::progress
 ```namespace
-String Char Nat
+String Char Nat Lean.Elab.Tactic
 ```
 ```exceptions
 String.revFindAux String.extract.go₂ String.substrEq.loop String.casesOn
@@ -96,6 +127,136 @@ Nat.le.below.rec
 Nat.le.below.recOn
 Nat.le.below.refl
 Nat.le.below.casesOn
+```
+
+```exceptions
+Lean.Elab.Tactic.evalUnfold.go
+Lean.Elab.Tactic.dsimpLocation.go
+Lean.Elab.Tactic.withCollectingNewGoalsFrom.go
+Lean.Elab.Tactic.evalRunTac.unsafe_impl_1
+Lean.Elab.Tactic.evalRunTac.unsafe_1
+Lean.Elab.Tactic.evalTactic.handleEx
+Lean.Elab.Tactic.simpLocation.go
+Lean.Elab.Tactic.instToSnapshotTreeTacticParsedSnapshot.go
+Lean.Elab.Tactic.dsimpLocation'.go
+Lean.Elab.Tactic.withRWRulesSeq.go
+Lean.Elab.Tactic.runTermElab.go
+Lean.Elab.Tactic.getMainGoal.loop
+Lean.Elab.Tactic.elabSimpArgs.isSimproc?
+Lean.Elab.Tactic.elabSimpArgs.resolveSimpIdTheorem?
+Lean.Elab.Tactic.tactic.dbg_cache
+Lean.Elab.Tactic.tactic.simp.trace
+Lean.Elab.Tactic.liftMetaTacticAux
+```
+
+```exceptions
+
+Lean.Elab.Tactic.elabSetOption
+Lean.Elab.Tactic.evalSeq1
+Lean.Elab.Tactic.evalSimp
+Lean.Elab.Tactic.evalSpecialize
+Lean.Elab.Tactic.evalTacticAt
+Lean.Elab.Tactic.evalSimpAll
+Lean.Elab.Tactic.evalIntro.introStep
+Lean.Elab.Tactic.evalDone
+Lean.Elab.Tactic.evalRevert
+Lean.Elab.Tactic.evalRight
+Lean.Elab.Tactic.evalUnfold
+Lean.Elab.Tactic.evalConstructor
+Lean.Elab.Tactic.evalTacticCDot
+Lean.Elab.Tactic.evalTraceMessage
+Lean.Elab.Tactic.evalClear
+Lean.Elab.Tactic.evalIntroMatch
+Lean.Elab.Tactic.evalInduction
+Lean.Elab.Tactic.evalApply
+Lean.Elab.Tactic.evalUnknown
+Lean.Elab.Tactic.evalRefl
+Lean.Elab.Tactic.evalTactic.throwExs
+Lean.Elab.Tactic.evalDSimp
+Lean.Elab.Tactic.evalSepTactics.goEven
+Lean.Elab.Tactic.evalAllGoals
+Lean.Elab.Tactic.evalSplit
+Lean.Elab.Tactic.evalInjection
+Lean.Elab.Tactic.evalParen
+Lean.Elab.Tactic.evalFocus
+Lean.Elab.Tactic.evalLeft
+Lean.Elab.Tactic.evalRotateRight
+Lean.Elab.Tactic.evalWithReducible
+Lean.Elab.Tactic.evalTactic.expandEval
+Lean.Elab.Tactic.evalTraceState
+Lean.Elab.Tactic.evalCase'
+Lean.Elab.Tactic.evalSepTactics.goOdd
+Lean.Elab.Tactic.evalWithReducibleAndInstances
+Lean.Elab.Tactic.evalTacticSeqBracketed
+Lean.Elab.Tactic.evalTactic.eval
+Lean.Elab.Tactic.evalAlt
+Lean.Elab.Tactic.evalGeneralize
+Lean.Elab.Tactic.evalRewriteSeq
+Lean.Elab.Tactic.evalSleep
+Lean.Elab.Tactic.evalDSimpTrace
+Lean.Elab.Tactic.evalReplace
+Lean.Elab.Tactic.evalOpen
+Lean.Elab.Tactic.evalAssumption
+Lean.Elab.Tactic.evalSepTactics
+Lean.Elab.Tactic.evalWithUnfoldingAll
+Lean.Elab.Tactic.evalMatch
+Lean.Elab.Tactic.evalRepeat1'
+Lean.Elab.Tactic.evalFailIfSuccess
+Lean.Elab.Tactic.evalRename
+Lean.Elab.Tactic.evalFirst.loop
+Lean.Elab.Tactic.evalSimpTrace
+Lean.Elab.Tactic.evalFirst
+Lean.Elab.Tactic.evalSubstVars
+Lean.Elab.Tactic.evalRunTac
+Lean.Elab.Tactic.evalSymmSaturate
+Lean.Elab.Tactic.evalWithAnnotateState
+Lean.Elab.Tactic.evalTacticAtRaw
+Lean.Elab.Tactic.evalDbgTrace
+Lean.Elab.Tactic.evalSubst
+Lean.Elab.Tactic.evalNativeDecide
+Lean.Elab.Tactic.evalCalc
+Lean.Elab.Tactic.evalCase
+Lean.Elab.Tactic.evalRepeat'
+Lean.Elab.Tactic.evalRefine
+Lean.Elab.Tactic.evalContradiction
+Lean.Elab.Tactic.evalSymm
+Lean.Elab.Tactic.evalInjections
+Lean.Elab.Tactic.evalExact
+Lean.Elab.Tactic.evalRotateLeft
+Lean.Elab.Tactic.evalFail
+Lean.Elab.Tactic.evalTactic
+Lean.Elab.Tactic.evalSimpAllTrace
+Lean.Elab.Tactic.evalRefine'
+Lean.Elab.Tactic.evalChoice
+Lean.Elab.Tactic.evalInduction.checkTargets
+Lean.Elab.Tactic.evalIntro
+Lean.Elab.Tactic.evalAnyGoals
+Lean.Elab.Tactic.evalCases
+Lean.Elab.Tactic.evalDelta
+Lean.Elab.Tactic.evalDecide
+Lean.Elab.Tactic.evalChoiceAux
+Lean.Elab.Tactic.evalTacticSeq
+Lean.Elab.Tactic.evalCheckpoint
+Lean.Elab.Tactic.evalRenameInaccessibles
+Lean.Elab.Tactic.evalIntros
+Lean.Elab.Tactic.evalApplyLikeTactic
+Lean.Elab.Tactic.evalSkip
+Lean.Elab.Tactic.evalCalc.throwFailed
+Lean.Elab.Tactic.evalSubstEqs
+Lean.Elab.Tactic.evalTacticSeq1Indented
+```
+
+```exceptions
+List.tacticSizeOf_list_dec
+Lean.Parser.Tactic.tacticRefine_lift_
+Lean.Parser.Tactic.tacticRefine_lift'_
+Array.tacticArray_mem_dec
+Lean.Parser.Tactic.normCast0
+tacticClean_wf
+Lean.Parser.Tactic.nestedTactic
+Lean.Parser.Tactic.unknown
+Lean.Parser.Tactic.paren
+tacticDecreasing_trivial_pre_omega
 ```
 
 :::
