Manual/Elaboration.lean
@@ -11,7 +11,7 @@ set_option pp.rawOnError true
 :::planned
 
 
- * Describe the roles of the kernel, the interpreter, the compiler, the {deftech key:="elaborate"}[elaborator], and how they interact
+ * Describe the roles of the {deftech}_kernel_, the interpreter, the compiler, the {deftech key:="elaborate"}[elaborator], and how they interact
  * Sketch the pipeline (parser -> command elaborator (with macro expansion) -> term elaborator (with macro expansion) -> ...
  * Cost model for programs - what data is present at which stage?
 
