Manual/Meta.lean
@@ -11,11 +11,13 @@ import SubVerso.Highlighting
 import SubVerso.Examples
 
 import Manual.Meta.Basic
+import Manual.Meta.CustomStyle
 import Manual.Meta.Example
 import Manual.Meta.Figure
 import Manual.Meta.Lean
 import Manual.Meta.Marginalia
 import Manual.Meta.Syntax
+import Manual.Meta.Tactics
 
 open Lean Elab
 open Verso ArgParse Doc Elab Genre.Manual Html Code Highlighted.WebAssets
