Manual/Meta/CustomStyle.lean
@@ -1,0 +1,35 @@
+import VersoManual
+import Lean.Data.Json
+
+open Verso Doc Elab Output Html Code
+open Verso.Genre Manual
+open Verso.ArgParse
+open Lean
+
+namespace Manual
+
+
+def Block.CSS : Block where
+  name := `Manual.CSS
+
+@[code_block_expander CSS]
+def CSS : CodeBlockExpander
+  | args, str => do
+    let () ← ArgParse.done.run args
+    pure #[← `(Doc.Block.other {Block.CSS with data := ToJson.toJson (α := String) $(quote str.getString)} #[])]
+
+@[block_extension Manual.CSS]
+def CSS.descr : BlockDescr where
+  traverse _ _ _ := pure none
+  toTeX := none
+  toHtml :=
+    open Verso.Output.Html in
+    some <| fun _ _ _ data _ => do
+      match FromJson.fromJson? data with
+      | .error err =>
+        HtmlT.logError <| "Couldn't deserialize CSS while rendering HTML: " ++ err
+        pure .empty
+      | .ok (css : String) =>
+        pure {{
+          <style>{{css}}</style>
+        }}
