Manual/Meta/Tactics.lean
@@ -1,0 +1,638 @@
+import Lean.Elab.Term
+import Lean.Elab.Tactic
+
+import Verso.Code.Highlighted
+import Verso.Doc.ArgParse
+import Verso.Doc.Suggestion
+import SubVerso.Highlighting.Code
+import VersoManual
+
+import Manual.Meta.Basic
+import Manual.Meta.PPrint
+import Manual.Meta.Lean
+import Manual.Meta.Lean.Scopes
+
+namespace Manual
+
+open Lean Elab Term Tactic
+open Verso ArgParse Doc Elab Genre.Manual Html Code Highlighted.WebAssets
+open Manual.Meta.Lean.Scopes
+open SubVerso.Highlighting
+
+structure TacticOutputConfig where
+  «show» : Bool := true
+  severity : Option MessageSeverity
+  summarize : Bool
+  whitespace : GuardMsgs.WhitespaceMode
+
+def TacticOutputConfig.parser [Monad m] [MonadInfoTree m] [MonadLiftT CoreM m] [MonadEnv m] [MonadError m] : ArgParse m TacticOutputConfig :=
+  TacticOutputConfig.mk <$>
+    ((·.getD true) <$> .named `show .bool true) <*>
+    .named `severity LeanOutputConfig.parser.sev true <*>
+    ((·.getD false) <$> .named `summarize .bool true) <*>
+    ((·.getD .exact) <$> .named `whitespace LeanOutputConfig.parser.ws true)
+
+
+def checkTacticExample (goal : Term) (proofPrefix : Syntax) (tactic : Syntax) (pre : TSyntax `str) (post : TSyntax `str) : TermElabM Unit := do
+  let statement ← elabType goal
+  let mv ← Meta.mkFreshExprMVar (some statement)
+  let Expr.mvar mvarId := mv
+    | throwError "Not an mvar!"
+  -- `runTactic` is too specialized for this purpose - we need to capture the unsolved goals, not
+  -- throw them as an exception. This code is adapted from `runTactic`.
+  let remainingGoals ← withInfoHole mvarId <| Tactic.run mvarId do
+    withoutTacticIncrementality true <|
+    withTacticInfoContext proofPrefix do
+      -- also put an info node on the `by` keyword specifically -- the token may be `canonical` and thus shown in the info
+      -- view even though it is synthetic while a node like `tacticCode` never is (#1990)
+      evalTactic proofPrefix
+    synthesizeSyntheticMVars (postpone := .no)
+  -- `runTactic` extraction done. Now prettyprint the proof state.
+  let st1 := goalsToMessageData remainingGoals
+  --logInfoAt proofPrefix st1
+  let goodPre ← (← addMessageContext st1).toString
+  if pre.getString != goodPre then
+    logErrorAt pre m!"Mismatch. Expected {indentD goodPre}\n but got {indentD pre.getString}"
+  -- Run the example
+  let remainingGoals' ← Tactic.run mvarId do
+    withoutTacticIncrementality true <|
+    withTacticInfoContext tactic do
+      set (Tactic.State.mk remainingGoals)
+      evalTactic tactic
+  let st2 := goalsToMessageData remainingGoals'
+  --logInfoAt tactic st2
+  let goodPost ← (← addMessageContext st2).toString
+  if post.getString != goodPost then
+    logErrorAt post m!"Mismatch. Expected {indentD goodPost}\n but got {indentD post.getString}"
+
+open Lean.Elab.Tactic.GuardMsgs in
+def checkTacticExample'
+    (goal : Expr) (proofPrefix : Syntax) (tactic : Syntax)
+    (pre : TSyntax `str) (post : TSyntax `str)
+    (output : Option (TSyntax `str × TacticOutputConfig)) :
+    TermElabM
+      (Array (Highlighted.Goal Highlighted) ×
+        Array (Highlighted.Goal Highlighted) ×
+        Highlighted ×
+        MessageSeverity) := do
+  let mv ← Meta.mkFreshExprMVar (some goal)
+  let Expr.mvar mvarId := mv
+    | throwError "Not an mvar!"
+  -- `runTactic` is too specialized for this purpose - we need to capture the unsolved goals, not
+  -- throw them as an exception. This code is adapted from `runTactic`.
+  let ((remainingGoals, _setupMsgs), preTree) ← withInfoTreeContext (mkInfoTree := mkInfoTree `leanInline (← getRef)) do
+    let initMsgs ← Core.getMessageLog
+    try
+      Core.resetMessageLog
+      let remainingGoals ←
+        withInfoHole mvarId <| Tactic.run mvarId <|
+        withoutTacticIncrementality true <|
+        withTacticInfoContext proofPrefix do
+          -- also put an info node on the `by` keyword specifically -- the token may be `canonical` and thus shown in the info
+          -- view even though it is synthetic while a node like `tacticCode` never is (#1990)
+          evalTactic proofPrefix
+      synthesizeSyntheticMVars (postpone := .no)
+      let msgs ← Core.getMessageLog
+      pure (remainingGoals, msgs)
+    finally Core.setMessageLog initMsgs
+
+
+  -- `runTactic` extraction done. Now prettyprint the proof state.
+  let st1 := goalsToMessageData remainingGoals
+  --logInfoAt proofPrefix st1
+  let goodPre ← (← addMessageContext st1).toString
+  if pre.getString.trim != goodPre.trim then
+    Verso.Doc.Suggestion.saveSuggestion pre (goodPre.take 30 ++ "…") (goodPre ++ "\n")
+    logErrorAt pre m!"Mismatch. Expected {indentD goodPre}\n but got {indentD pre.getString}"
+
+  let ci : ContextInfo := {
+    env := ← getEnv, fileMap := ← getFileMap, ngen := ← getNGen,
+    mctx := ← getMCtx, options := ← getOptions,
+    currNamespace := ← getCurrNamespace, openDecls := ← getOpenDecls
+  }
+  let hlPre ← highlightProofState ci remainingGoals (PersistentArray.empty.push preTree)
+
+  -- Run the example
+  let ((remainingGoals', msgs), postTree) ← withInfoTreeContext (mkInfoTree := mkInfoTree `leanInline (← getRef)) do
+    let initMsgs ← Core.getMessageLog
+    try
+      Core.resetMessageLog
+      let remainingGoals' ← Tactic.run mvarId <|
+        withoutTacticIncrementality true <|
+        withTacticInfoContext tactic do
+          set (Tactic.State.mk remainingGoals)
+          evalTactic tactic
+      let msgs ← Core.getMessageLog
+      pure (remainingGoals', msgs)
+    finally Core.setMessageLog initMsgs
+  let st2 := goalsToMessageData remainingGoals'
+  --logInfoAt tactic st2
+  let goodPost ← (← addMessageContext st2).toString
+
+  if post.getString.trim != goodPost.trim then
+    Verso.Doc.Suggestion.saveSuggestion post (goodPost.take 30 ++ "…") (goodPost ++ "\n")
+    logErrorAt post m!"Mismatch. Expected {indentD goodPost}\n but got {indentD post.getString}"
+
+  let ci : ContextInfo := { ci with
+    mctx := ← getMCtx
+  }
+  let hlPost ← highlightProofState ci remainingGoals' (PersistentArray.empty.push postTree)
+
+  -- TODO suppress proof state bubbles here, at least as an option - `Inline.lean` needs to take that as an argument
+  let hlTac ← highlight tactic msgs.toArray (PersistentArray.empty.push postTree)
+  let outSev ← id <| do -- This 'id' is needed so that `return` in the `do` goes here
+    if let some (wantedOut, config) := output then
+      let processed ← msgs.toArray.mapM fun msg => do
+            let head := if msg.caption != "" then msg.caption ++ ":\n" else ""
+            let txt := withNewline <| head ++ (← msg.data.toString)
+            pure (msg.severity, txt)
+      for (sev, txt) in processed do
+        if mostlyEqual config.whitespace wantedOut.getString txt then
+          if let some s := config.severity then
+            if s != sev then
+              throwErrorAt wantedOut s!"Expected severity {sevStr s}, but got {sevStr sev}"
+          return sev
+      for (_, m) in processed do
+        Verso.Doc.Suggestion.saveSuggestion wantedOut (m.take 30 ++ "…") m
+      throwErrorAt wantedOut "Didn't match - expected one of: {indentD (toMessageData <| processed.map (·.2))}\nbut got:{indentD (toMessageData wantedOut.getString)}"
+    else pure .information
+
+  return (hlPre, hlPost, hlTac, outSev)
+where
+  withNewline (str : String) := if str == "" || str.back != '\n' then str ++ "\n" else str
+
+  sevStr : MessageSeverity → String
+    | .error => "error"
+    | .information => "information"
+    | .warning => "warning"
+
+  mostlyEqual (ws : WhitespaceMode) (s1 s2 : String) : Bool :=
+    ws.apply s1.trim == ws.apply s2.trim
+
+  mkInfoTree (elaborator : Name) (stx : Syntax) (trees : PersistentArray InfoTree) : TermElabM InfoTree := do
+    let tree := InfoTree.node (Info.ofCommandInfo { elaborator, stx }) trees
+    let ctx := PartialContextInfo.commandCtx {
+      env := ← getEnv, fileMap := ← getFileMap, mctx := {}, currNamespace := ← getCurrNamespace,
+      openDecls := ← getOpenDecls, options := ← getOptions, ngen := ← getNGen
+    }
+    return InfoTree.context ctx tree
+
+  modifyInfoTrees {m} [Monad m] [MonadInfoTree m] (f : PersistentArray InfoTree → PersistentArray InfoTree) : m Unit :=
+    modifyInfoState fun s => { s with trees := f s.trees }
+
+  -- TODO - consider how to upstream this
+  withInfoTreeContext {m α} [Monad m] [MonadInfoTree m] [MonadFinally m] (x : m α) (mkInfoTree : PersistentArray InfoTree → m InfoTree) : m (α × InfoTree) := do
+    let treesSaved ← getResetInfoTrees
+    MonadFinally.tryFinally' x fun _ => do
+      let st    ← getInfoState
+      let tree  ← mkInfoTree st.trees
+      modifyInfoTrees fun _ => treesSaved.push tree
+      pure tree
+
+
+open Command
+
+-- TODO: This code would be much nicer if genres could impose custom elaboration contexts as well.
+-- As things are, this seems to require hygiene-bending and environment mutation (basically the
+-- fluid-let trick, in the absence of syntax parameters), which is icky and tricky and error-prone.
+
+structure TacticExampleContext where
+  goal : Option Expr := none
+  setup : Option Syntax := none
+  pre : Option (TSyntax `str) := none
+  preName : Ident
+  tactic : Option Syntax := none
+  tacticName : Ident
+  post : Option (TSyntax `str) := none
+  postName : Ident
+  output : Option (TSyntax `str × TacticOutputConfig) := none
+  outputSeverityName : Ident
+
+initialize tacticExampleCtx : Lean.EnvExtension (Option TacticExampleContext) ←
+  Lean.registerEnvExtension (pure none)
+
+def startExample [Monad m] [MonadEnv m] [MonadError m] [MonadQuotation m] [MonadRef m] : m Unit := do
+  match tacticExampleCtx.getState (← getEnv) with
+  | some _ => throwError "Can't initialize - already in a context"
+  | none =>
+    let preName ← mkFreshIdent (← getRef)
+    let tacticName ← mkFreshIdent (← getRef)
+    let postName ← mkFreshIdent (← getRef)
+    let outputSeverityName ← mkFreshIdent (← getRef)
+    modifyEnv fun env =>
+      tacticExampleCtx.setState env (some {preName, tacticName, postName, outputSeverityName})
+
+def saveGoal [Monad m] [MonadEnv m] [MonadError m] (goal : Expr) : m Unit := do
+  match tacticExampleCtx.getState (← getEnv) with
+  | none => throwError "Can't set goal - not in a tactic example"
+  | some st =>
+    match st.goal with
+    | none => modifyEnv fun env => tacticExampleCtx.setState env (some {st with goal := goal})
+    | some _ => throwError "Goal already specified"
+
+def saveSetup [Monad m] [MonadEnv m] [MonadError m] (setup : Syntax) : m Unit := do
+  match tacticExampleCtx.getState (← getEnv) with
+  | none => throwError "Can't set setup - not in a tactic example"
+  | some st =>
+    match st.setup with
+    | none => modifyEnv fun env => tacticExampleCtx.setState env (some {st with setup := setup})
+    | some _ => throwError "Setup already specified"
+
+def saveTactic [Monad m] [MonadEnv m] [MonadError m] (tactic : Syntax) : m Ident := do
+  match tacticExampleCtx.getState (← getEnv) with
+  | none => throwError "Can't set tactic step - not in a tactic example"
+  | some st =>
+    match st.tactic with
+    | some _ => throwError "Tactic step already specified"
+    | none =>
+      modifyEnv fun env => tacticExampleCtx.setState env (some {st with tactic := tactic})
+      return st.tacticName
+
+def savePre [Monad m] [MonadEnv m] [MonadLog m] [MonadRef m] [MonadError m] [AddMessageContext m] [MonadOptions m] (pre : TSyntax `str) : m Ident := do
+  match tacticExampleCtx.getState (← getEnv) with
+  | none => throwError "Can't set pre-state - not in a tactic example"
+  | some st =>
+    match st.pre with
+    | none =>
+      modifyEnv fun env => tacticExampleCtx.setState env (some {st with pre := pre})
+    | some _ =>
+      logErrorAt (← getRef) "Pre-state already specified"
+    return st.preName
+
+def saveOutput [Monad m] [MonadEnv m] [MonadLog m] [MonadRef m] [MonadError m] [AddMessageContext m] [MonadOptions m] (output : TSyntax `str) (options : TacticOutputConfig) : m Ident := do
+  match tacticExampleCtx.getState (← getEnv) with
+  | none => throwError "Can't set expected output - not in a tactic example"
+  | some st =>
+    match st.output with
+    | none =>
+      modifyEnv fun env => tacticExampleCtx.setState env (some {st with output := (output, options)})
+    | some _ =>
+      logErrorAt (← getRef) "Expected output already specified"
+    return st.outputSeverityName
+
+
+def savePost [Monad m] [MonadEnv m] [MonadLog m] [MonadRef m] [MonadError m] [AddMessageContext m] [MonadOptions m] (post : TSyntax `str) : m Ident := do
+  match tacticExampleCtx.getState (← getEnv) with
+  | none => throwError "Can't set post-state - not in a tactic example"
+  | some st =>
+    match st.post with
+    | none =>
+      modifyEnv fun env => tacticExampleCtx.setState env (some {st with post := post})
+    | some _ =>
+      logErrorAt (← getRef) "Post-state already specified"
+    return st.postName
+
+
+def endExample (body : TSyntax `term) : DocElabM (TSyntax `term) := do
+  match tacticExampleCtx.getState (← getEnv) with
+  | none => throwErrorAt body "Can't end examples - never started"
+  | some {goal, setup, pre, preName, tactic, tacticName, post, postName, output, outputSeverityName} =>
+    modifyEnv fun env =>
+      tacticExampleCtx.setState env none
+    let some goal := goal
+      | throwErrorAt body "No goal specified"
+    let some setup := setup
+      | throwErrorAt body "No setup specified"
+    let some pre := pre
+      | throwErrorAt body "No pre-state specified"
+    let some tactic := tactic
+      | throwErrorAt body "No tactic specified"
+    let some post := post
+      | throwErrorAt body "No post-state specified"
+
+    let (hlPre, hlPost, hlTactic, outputSeverity) ← checkTacticExample' goal setup tactic pre post output
+
+    `(let $preName : Array (Highlighted.Goal Highlighted) := $(quote hlPre)
+      let $postName : Array (Highlighted.Goal Highlighted) := $(quote hlPost)
+      let $tacticName : Highlighted := $(quote hlTactic)
+      let $outputSeverityName : MessageSeverity := $(quote outputSeverity)
+      $body)
+
+@[directive_expander tacticExample]
+def tacticExample : DirectiveExpander
+ | args, blocks => do
+    ArgParse.done.run args
+    startExample
+    let body ← blocks.mapM elabBlock
+    let body' ← `(Verso.Doc.Block.concat #[$body,*]) >>= endExample
+    pure #[body']
+
+
+structure TacticGoalConfig where
+  «show» : Bool
+
+def TacticGoalConfig.parse [Monad m] [MonadInfoTree m] [MonadLiftT CoreM m] [MonadEnv m] [MonadError m] : ArgParse m TacticGoalConfig :=
+  TacticGoalConfig.mk <$> ((·.getD true) <$> .named `show .bool true)
+
+@[role_expander goal]
+def goal : RoleExpander
+  | args, inlines => do
+    let config ← TacticGoalConfig.parse.run args
+    let #[arg] := inlines
+      | throwError "Expected exactly one argument"
+    let `(inline|code{ $term:str }) := arg
+      | throwErrorAt arg "Expected code literal with the example name"
+    let altStr ← parserInputString term
+
+    match Parser.runParserCategory (← getEnv) `term altStr (← getFileName) with
+    | .error e => throwErrorAt term e
+    | .ok stx =>
+      let (newMsgs, tree) ← withInfoTreeContext (mkInfoTree := mkInfoTree `leanInline (← getRef)) do
+        let initMsgs ← Core.getMessageLog
+        try
+          Core.resetMessageLog
+          let goalExpr ← runWithOpenDecls <| runWithVariables fun _ => Elab.Term.elabTerm stx none
+          saveGoal goalExpr
+          Core.getMessageLog
+        finally
+          Core.setMessageLog initMsgs
+
+
+      for msg in newMsgs.toArray do
+        logMessage msg
+
+      -- TODO msgs
+      let hls := (← highlight stx #[] (PersistentArray.empty.push tree))
+
+      if config.show then
+        -- Just emit a normal Lean node - no need to do anything special with the rendered result
+        pure #[← `(Inline.other {Inline.lean with data := ToJson.toJson $(quote hls)} #[Inline.code $(quote term.getString)])]
+      else
+        pure #[]
+where
+  mkInfoTree (elaborator : Name) (stx : Syntax) (trees : PersistentArray InfoTree) : DocElabM InfoTree := do
+    let tree := InfoTree.node (Info.ofCommandInfo { elaborator, stx }) trees
+    let ctx := PartialContextInfo.commandCtx {
+      env := ← getEnv, fileMap := ← getFileMap, mctx := {}, currNamespace := ← getCurrNamespace,
+      openDecls := ← getOpenDecls, options := ← getOptions, ngen := ← getNGen
+    }
+    return InfoTree.context ctx tree
+
+  modifyInfoTrees {m} [Monad m] [MonadInfoTree m] (f : PersistentArray InfoTree → PersistentArray InfoTree) : m Unit :=
+    modifyInfoState fun s => { s with trees := f s.trees }
+
+  -- TODO - consider how to upstream this
+  withInfoTreeContext {m α} [Monad m] [MonadInfoTree m] [MonadFinally m] (x : m α) (mkInfoTree : PersistentArray InfoTree → m InfoTree) : m (α × InfoTree) := do
+    let treesSaved ← getResetInfoTrees
+    MonadFinally.tryFinally' x fun _ => do
+      let st    ← getInfoState
+      let tree  ← mkInfoTree st.trees
+      modifyInfoTrees fun _ => treesSaved.push tree
+      pure tree
+
+
+open Lean.Parser in
+@[code_block_expander setup]
+def setup : CodeBlockExpander
+  | args, str => do
+    let () ← ArgParse.done.run args
+
+    let altStr ← parserInputString str
+
+    let p := andthen ⟨{}, whitespace⟩ <| andthen {fn := (fun _ => (·.pushSyntax (mkIdent `tacticSeq)))} (parserOfStack 0)
+    match runParser (← getEnv) (← getOptions) p altStr (← getFileName) with
+    | .error es =>
+      for (pos, msg) in es do
+        log (severity := .error) (mkErrorStringWithPos  "<setup>" pos msg)
+      throwErrorAt str "Failed to parse setup"
+    | .ok stx =>
+      saveSetup stx
+      pure #[]
+
+
+open Lean.Parser in
+@[code_block_expander tacticOutput]
+def tacticOutput : CodeBlockExpander
+  | args, str => do
+    let opts ← TacticOutputConfig.parser.run args
+    let outputSeverityName ← saveOutput str opts
+
+    if opts.show then
+      return #[← `(Block.other {Block.leanOutput with data := ToJson.toJson ($outputSeverityName, $(quote str.getString), $(quote opts.summarize))} #[Block.code $(quote str.getString)])]
+    else
+      return #[]
+
+
+open Lean.Parser in
+@[code_block_expander tacticStep]
+def tacticStep : CodeBlockExpander
+  | args, str => do
+    let () ← ArgParse.done.run args
+
+    let altStr ← parserInputString str
+
+    let p := andthen ⟨{}, whitespace⟩ <| andthen {fn := (fun _ => (·.pushSyntax (mkIdent `tacticSeq)))} (parserOfStack 0)
+    match runParser (← getEnv) (← getOptions) p altStr (← getFileName) with
+    | .error es =>
+      for (pos, msg) in es do
+        log (severity := .error) (mkErrorStringWithPos  "<setup>" pos msg)
+      throwErrorAt str "Failed to parse tactic step"
+    | .ok stx =>
+      let hlTac ← saveTactic stx
+      pure #[← `(Block.other {Block.lean with data := ToJson.toJson (α := Highlighted) $hlTac} #[Block.code $(quote str.getString)])]
+
+open Lean.Parser in
+@[role_expander tacticStep]
+def tacticStepInline : RoleExpander
+  | args, inlines => do
+    let () ← ArgParse.done.run args
+    let #[arg] := inlines
+      | throwError "Expected exactly one argument"
+    let `(inline|code{ $tacStr:str }) := arg
+      | throwErrorAt arg "Expected code literal with the example name"
+
+    let altStr ← parserInputString tacStr
+
+    let p := andthen ⟨{}, whitespace⟩ <| andthen {fn := (fun _ => (·.pushSyntax (mkIdent `tacticSeq)))} (parserOfStack 0)
+    match runParser (← getEnv) (← getOptions) p altStr (← getFileName) with
+    | .error es =>
+      for (pos, msg) in es do
+        log (severity := .error) (mkErrorStringWithPos  "<setup>" pos msg)
+      throwErrorAt arg "Failed to parse tactic step"
+    | .ok stx =>
+      let hlTac ← saveTactic stx
+
+      pure #[← `(Inline.other {Inline.lean with data := ToJson.toJson (α := Highlighted) $hlTac} #[Inline.code $(quote tacStr.getString)])]
+
+def Block.proofState : Block where
+  name := `Manual.proofState
+
+structure ProofStateOptions where
+  tag : Option String := none
+
+
+def ProofStateOptions.parse [Monad m] [MonadInfoTree m] [MonadLiftT CoreM m] [MonadEnv m] [MonadError m] : ArgParse m ProofStateOptions :=
+  ProofStateOptions.mk <$> .named `tag .string true
+
+
+open Lean.Parser in
+/--
+Show a proof state in the text. The proof goal is expected as a documentation comment immediately
+prior to tactics.
+-/
+@[code_block_expander proofState]
+def proofState : CodeBlockExpander
+  | args, str => do
+    let opts ← ProofStateOptions.parse.run args
+    let altStr ← parserInputString str
+    let p :=
+      node nullKind <|
+      andthen ⟨{}, whitespace⟩ <|
+      andthen termParser <|
+      andthen ⟨{}, whitespace⟩ <|
+      andthen ":=" <| andthen ⟨{}, whitespace⟩ <| andthen "by" <|
+      andthen ⟨{}, whitespace⟩ <|
+      andthen (andthen {fn := (fun _ => (·.pushSyntax (mkIdent `tacticSeq)))} (parserOfStack 0)) <|
+      optional <|
+        andthen  ⟨{}, whitespace⟩ <|
+        Command.docComment
+    match runParser (← getEnv) (← getOptions) p altStr (← getFileName) with
+    | .error es =>
+      for (pos, msg) in es do
+        log (severity := .error) (mkErrorStringWithPos  "<setup>" pos msg)
+      throwErrorAt str "Failed to parse config (expected goal term, followed by ':=', 'by', and tactics, with optional docstring)"
+    | .ok stx =>
+      let goalStx := stx[0]
+      let tacticStx := stx[4]
+      let desired :=
+        match stx[5][0] with
+        | .missing => none
+        | other => some (⟨other⟩ : TSyntax `Lean.Parser.Command.docComment)
+      let goalExpr ← runWithOpenDecls <| runWithVariables fun _ => Elab.Term.elabTerm goalStx none
+      let mv ← Meta.mkFreshExprMVar (some goalExpr)
+        let Expr.mvar mvarId := mv
+          | throwError "Not an mvar!"
+      let (remainingGoals, infoTree) ← withInfoTreeContext (mkInfoTree := mkInfoTree `proofState (← getRef)) do
+            Tactic.run mvarId <|
+            withoutTacticIncrementality true <|
+            withTacticInfoContext tacticStx do
+              evalTactic tacticStx
+      synthesizeSyntheticMVars (postpone := .no)
+      let ci : ContextInfo := {
+        env := ← getEnv, fileMap := ← getFileMap, ngen := ← getNGen,
+        mctx := ← getMCtx, options := ← getOptions,
+        currNamespace := ← getCurrNamespace, openDecls := ← getOpenDecls
+      }
+      let hlState ← highlightProofState ci remainingGoals (PersistentArray.empty.push infoTree)
+      let st := goalsToMessageData remainingGoals
+      --logInfoAt proofPrefix st1
+      let stStr ← (← addMessageContext st).toString
+      if let some s := desired then
+        if stStr.trim != s.getDocString.trim then
+          logErrorAt s m!"Expected: {indentD stStr}\n\nGot: {indentD s.getDocString}"
+          Verso.Doc.Suggestion.saveSuggestion s (stStr.take 30 ++ "…") ("/--\n" ++ stStr ++ "\n-/\n")
+      pure #[← `(Doc.Block.other {Block.proofState with data := ToJson.toJson (α := Option String × Array (Highlighted.Goal Highlighted)) ($(quote opts.tag), $(quote hlState))} #[Doc.Block.code $(quote stStr)])]
+
+where
+  mkInfoTree (elaborator : Name) (stx : Syntax) (trees : PersistentArray InfoTree) : DocElabM InfoTree := do
+    let tree := InfoTree.node (Info.ofCommandInfo { elaborator, stx }) trees
+    let ctx := PartialContextInfo.commandCtx {
+      env := ← getEnv, fileMap := ← getFileMap, mctx := {}, currNamespace := ← getCurrNamespace,
+      openDecls := ← getOpenDecls, options := ← getOptions, ngen := ← getNGen
+    }
+    return InfoTree.context ctx tree
+
+  modifyInfoTrees {m} [Monad m] [MonadInfoTree m] (f : PersistentArray InfoTree → PersistentArray InfoTree) : m Unit :=
+    modifyInfoState fun s => { s with trees := f s.trees }
+
+  -- TODO - consider how to upstream this
+  withInfoTreeContext {m α} [Monad m] [MonadInfoTree m] [MonadFinally m] (x : m α) (mkInfoTree : PersistentArray InfoTree → m InfoTree) : m (α × InfoTree) := do
+    let treesSaved ← getResetInfoTrees
+    MonadFinally.tryFinally' x fun _ => do
+      let st    ← getInfoState
+      let tree  ← mkInfoTree st.trees
+      modifyInfoTrees fun _ => treesSaved.push tree
+      pure tree
+
+
+
+
+def proofStateStyle := r#"
+.hl.lean.tactic-view {
+  white-space: collapse;
+}
+.hl.lean.tactic-view .tactic-state {
+  display: block;
+  left: 0;
+  padding: 0;
+  border: none;
+}
+
+.hl.lean.tactic-view .tactic-state .goal {
+  margin-top: 0.25em;
+  margin-bottom: 0.25em;
+}
+"#
+
+
+
+@[block_extension Manual.proofState]
+def proofState.descr : BlockDescr where
+  traverse id data content := do
+    match FromJson.fromJson? data (α := Option String × Array (Highlighted.Goal Highlighted)) with
+    | .error e => logError s!"Error deserializing proof state info: {e}"; pure none
+    | .ok (none, _) => pure none
+    | .ok (some t, v) =>
+      let path ← (·.path) <$> read
+      let _tag ← Verso.Genre.Manual.externalTag id path t
+      pure <| some <| Block.other {Block.proofState with id := some id, data := ToJson.toJson (α := (Option String × _)) (none, v)} content
+
+  toTeX := none
+  extraCss := [highlightingStyle, proofStateStyle]
+  extraJs := [highlightingJs]
+  extraJsFiles := [("popper.js", popper), ("tippy.js", tippy)]
+  extraCssFiles := [("tippy-border.css", tippy.border.css)]
+  toHtml :=
+    open Verso.Output.Html in
+    some <| fun _ _ id data _ => do
+      match FromJson.fromJson? (α := Option Tag × Array (Highlighted.Goal Highlighted)) data with
+      | .error err =>
+        HtmlT.logError <| "Couldn't deserialize proof state while rendering HTML: " ++ err
+        pure .empty
+      | .ok (_, goals) =>
+        let idAttr :=
+          if let some (_, t) := (← read).traverseState.externalTags.get? id then
+            #[("id", t)]
+          else #[]
+        pure {{
+          <div class="hl lean tactic-view">
+            <div class="tactic-state" {{idAttr}}>
+              {{← if goals.isEmpty then
+                  pure {{"All goals completed! 🐙"}}
+                else
+                  .seq <$> goals.mapIndexedM (fun ⟨i, _⟩ x => withCollapsedSubgoals .never <| x.toHtml (·.toHtml) i)}}
+            </div>
+          </div>
+        }}
+
+structure StateConfig where
+  tag : Option String := none
+  «show» : Bool := true
+
+def StateConfig.parse [Monad m] [MonadInfoTree m] [MonadLiftT CoreM m] [MonadEnv m] [MonadError m] : ArgParse m StateConfig :=
+  StateConfig.mk <$> .named `tag .string true <*> ((·.getD true) <$> .named `show .bool true)
+
+@[code_block_expander pre]
+def pre : CodeBlockExpander
+  | args, str => do
+    let opts ← StateConfig.parse.run args
+    let hlPre ← savePre str
+    -- The quote step here is to prevent the editor from showing document AST internals when the
+    -- cursor is on the code block
+    if opts.show then
+      pure #[← `(Doc.Block.other {Block.proofState with data := ToJson.toJson (α := Option String × Array (Highlighted.Goal Highlighted)) ($(quote opts.tag), $(hlPre))} #[Doc.Block.code $(quote str.getString)])]
+    else
+      pure #[]
+
+
+@[code_block_expander post]
+def post : CodeBlockExpander
+  | args, str => do
+    let opts ← StateConfig.parse.run args
+    let hlPost ← savePost str
+    -- The quote step here is to prevent the editor from showing document AST internals when the
+    -- cursor is on the code block
+    if opts.show then
+      pure #[← `(Doc.Block.other {Block.proofState with data := ToJson.toJson (α := Option String × Array (Highlighted.Goal Highlighted)) ($(quote opts.tag), $(hlPost))} #[Doc.Block.code $(quote str.getString)])]
+    else
+      pure #[]
