Manual/Simp.lean
@@ -1,0 +1,24 @@
+import VersoManual
+
+import Lean.Parser.Term
+
+import Manual.Meta
+
+open Verso.Genre Manual
+
+set_option pp.rawOnError true
+
+set_option linter.unusedVariables false
+
+#doc (Manual) "The Simplifier" =>
+%%%
+tag := "the-simplifier"
+%%%
+
+:::planned
+Describe {tactic}`simp` in detail, including:
+ * The concept of {tactic}`simp` normal form and its importance
+ * The `@[simp]` attribute
+ * Simprocs
+ * A comparison of how `simp` and `rw` use equality lemmas
+:::
