Manual/Tactics/Conv.lean
@@ -1,0 +1,251 @@
+import VersoManual
+
+import Lean.Parser.Term
+
+import Manual.Meta
+
+
+open Verso.Genre Manual
+
+set_option pp.rawOnError true
+
+set_option linter.unusedVariables false
+
+#doc (Manual) "Targeted Rewriting with {tactic}`conv`" =>
+
+
+The {tactic}`conv`, or conversion, tactic allows targeted rewriting within a goal.
+The argument to {tactic}`conv` is written in a separate language that interoperates with the main tactic language; it features commands to navigate to specific subterms within the goal along with commands that allow these subterms to be rewritten.
+{tactic}`conv` is useful when rewrites should only be applied in part of a goal (e.g. only on one side of an equality), rather than across the board, or when rewrites should be applied underneath a binder that prevents tactics like {tactic}`rw` from accessing the term.
+
+The conversion tactic language is very similar to the main tactic language: it uses the same proof states, tactics work primarily on the main goal and may either fail or succeed with a sequence of new goals, and macro expansion is interleaved with tactic execution.
+Unlike the main tactic language, in which tactics are intended to eventually solve goals, the {tactic}`conv` tactic is used to _change_ a goal so that it becomes amenable to further processing in the main tactic language.
+Goals that are intended to be rewritten with {tactic}`conv` are shown with a vertical bar instead of a turnstile.
+
+:::tactic "conv"
+:::
+
+::::example "Navigation and Rewriting with {tactic}`conv`"
+
+In this example, there are multiple instances of addition, and {tactic}`rw` would by default rewrite the first instance that it encounters.
+Using {tactic}`conv` to navigate to the specific subterm before rewriting leaves {tactic}`rw` no choice but to rewrite the correct term.
+
+```lean
+example (x y z : Nat) : x + (y + z) = (x + z) + y := by
+  conv =>
+    lhs
+    arg 2
+    rw [Nat.add_comm]
+  rw [Nat.add_assoc]
+```
+
+::::
+
+::::example "Rewriting Under Binders with {tactic}`conv`"
+
+In this example, addition occurs under binders, so {tactic}`rw` can't be used.
+However, after using {tactic}`conv` to navigate to the function body, it succeeds.
+The nested use of {tactic}`conv` causes control to return to the current position in the term after performing further coversions on one of its subterms.
+Because the goal is a reflexive equation after rewriting, {tactic}`conv` automatically closes it.
+
+```lean
+example : (fun (x y z : Nat) => x + (y + z)) = (fun x y z => (z + x) + y) := by
+  conv =>
+    lhs
+    intro x y z
+    conv =>
+      arg 2
+      rw [Nat.add_comm]
+    rw [← Nat.add_assoc]
+    arg 1
+    rw [Nat.add_comm]
+```
+
+::::
+
+# Control Structures
+
+
+:::conv first show := "first"
+:::
+
+:::conv convTry_ show := "try"
+:::
+
+:::conv «conv_<;>_» show:="<;>"
+:::
+
+:::conv convRepeat_ show := "repeat"
+:::
+
+:::conv skip show:= "skip"
+:::
+
+:::conv nestedConv show:= "{ ... }"
+:::
+
+:::conv paren show:= "( ... )"
+:::
+
+:::conv convDone show:= "done"
+:::
+
+# Goal Selection
+
+:::conv allGoals show:= "all_goals"
+:::
+
+:::conv anyGoals show:= "any_goals"
+:::
+
+:::conv case show:= "case ... => ..."
+:::
+
+:::conv case' show:= "case' ... => ..."
+:::
+
+:::conv «convNext__=>_» show:= "next ... => ..."
+:::
+
+:::conv focus show := "focus"
+:::
+
+:::conv «conv·._» show := ". ..."
+:::
+
+:::conv «conv·._» show := "· ..."
+:::
+
+:::conv failIfSuccess show := "fail_if_success"
+:::
+
+
+# Navigation
+
+:::conv lhs show:= "lhs"
+:::
+
+:::conv rhs show:= "rhs"
+:::
+
+:::conv fun show:= "fun"
+:::
+
+:::conv congr show:= "congr"
+:::
+
+:::conv arg show:= "arg [@]i"
+:::
+
+:::syntax Lean.Parser.Tactic.Conv.enterArg
+```grammar
+$i:num
+```
+```grammar
+@$i:num
+```
+```grammar
+$x:ident
+```
+:::
+
+:::conv «convEnter[_]» show := "enter"
+:::
+
+
+:::conv pattern show:= "pattern"
+:::
+
+:::conv ext show:= "ext"
+:::
+
+:::conv convArgs show := "args"
+:::
+
+:::conv convLeft show := "left"
+:::
+
+:::conv convRight show := "right"
+:::
+
+:::conv convIntro___ show := "intro"
+:::
+
+# Changing the Goal
+## Reduction
+
+:::conv whnf show:= "whnf"
+:::
+
+:::conv reduce show:= "reduce"
+:::
+
+:::conv zeta show:= "zeta"
+:::
+
+:::conv delta show:= "delta"
+:::
+
+:::conv unfold show:= "unfold"
+:::
+
+## Simplification
+:::conv simp show:= "simp"
+:::
+
+:::conv dsimp show:= "dsimp"
+:::
+
+:::conv simpMatch show:= "simp_match"
+:::
+
+## Rewriting
+
+
+:::conv change show:= "change"
+:::
+
+:::conv rewrite show:= "rewrite"
+:::
+
+:::conv convRw__ show := "rw"
+:::
+
+:::conv convErw_ show := "erw"
+:::
+
+:::conv convApply_ show := "apply"
+:::
+
+
+# Nested Tactics
+
+:::tactic Lean.Parser.Tactic.Conv.convTactic
+:::
+
+:::conv nestedTactic show:= "tactic"
+:::
+
+:::conv nestedTacticCore show:= "tactic'"
+:::
+
+:::tactic Lean.Parser.Tactic.Conv.convTactic show:= "conv'"
+:::
+
+:::conv convConvSeq show := "conv => ..."
+:::
+
+
+# Debugging Utilities
+
+:::conv convTrace_state show:= "trace_state"
+:::
+
+
+# Other
+
+:::conv convRfl show:= "rfl"
+:::
+
+:::conv normCast show := "norm_cast"
+:::
