Manual/Tactics/Reference.lean
@@ -1,0 +1,512 @@
+import VersoManual
+
+import Lean.Parser.Term
+
+import Manual.Meta
+
+
+open Verso.Genre Manual
+
+set_option pp.rawOnError true
+
+set_option linter.unusedVariables false
+
+#doc (Manual) "Tactic Reference" =>
+
+
+
+
+# Assumptions
+
+
+:::tactic Lean.Parser.Tactic.assumption
+:::
+
+
+:::tactic "apply_assumption"
+:::
+
+# Quantifiers
+
+:::tactic "exists"
+:::
+
+:::tactic "intro"
+:::
+
+
+:::tactic "intros"
+:::
+
+:::tactic Lean.Parser.Tactic.introMatch (show := "intro | ... => ... | ... => ...")
+:::
+
+:::tactic "rintro"
+:::
+
+
+# Relations
+
+:::planned
+ * Descriptions of the `symm` and `refl` and `trans` attributes
+:::
+
+:::tactic "rfl"
+:::
+
+:::tactic "rfl'"
+:::
+
+
+:::tactic Lean.Parser.Tactic.applyRfl
+:::
+
+:::tactic "symm"
+:::
+
+:::tactic "symm_saturate"
+:::
+
+
+:::tactic "calc"
+:::
+
+
+## Equality
+
+:::tactic "subst"
+:::
+
+:::tactic "subst_eqs"
+:::
+
+:::tactic "subst_vars"
+:::
+
+:::tactic "congr"
+:::
+
+:::tactic "eq_refl"
+:::
+
+:::tactic "ac_rfl"
+:::
+
+# Lemmas
+
+:::tactic "exact"
+:::
+
+:::tactic "apply"
+:::
+
+:::tactic "refine"
+:::
+
+:::tactic "refine'"
+:::
+
+:::tactic "solve_by_elim"
+:::
+
+
+:::tactic "apply_rules"
+:::
+
+# Falsehood
+
+:::tactic "exfalso"
+:::
+
+:::tactic "contradiction"
+:::
+
+:::tactic Lean.Parser.Tactic.falseOrByContra
+:::
+
+
+# Goal Management
+
+:::tactic "suffices"
+:::
+
+:::tactic "change"
+:::
+
+:::tactic Lean.Parser.Tactic.changeWith show:="change ... with ..."
+:::
+
+:::tactic "generalize"
+:::
+
+:::tactic "specialize"
+:::
+
+:::tactic "obtain"
+:::
+
+:::tactic "show"
+:::
+
+:::tactic Lean.Parser.Tactic.showTerm
+:::
+
+
+# Cast Management
+
+The tactics in this section make it easier avoid getting stuck on {deftech}_casts_, which are functions that coerce data from one type to another, such as converting a natural number to the corresponding integer.
+They are described in more detail in [_Simplifying Casts and Coercions_](https://arxiv.org/abs/2001.10594) by Robert Y. Lewis and Paul-Nicolas Madelaine.
+
+:::tactic Lean.Parser.Tactic.tacticNorm_cast_
+:::
+
+:::tactic Lean.Parser.Tactic.pushCast
+:::
+
+:::tactic Lean.Parser.Tactic.tacticExact_mod_cast_
+:::
+
+:::tactic Lean.Parser.Tactic.tacticApply_mod_cast_
+:::
+
+:::tactic Lean.Parser.Tactic.tacticRw_mod_cast___
+:::
+
+:::tactic Lean.Parser.Tactic.tacticAssumption_mod_cast
+:::
+
+
+
+
+# Extensionality
+
+
+:::tactic "ext"
+:::
+
+:::tactic Lean.Elab.Tactic.Ext.tacticExt1___
+:::
+
+:::tactic Lean.Elab.Tactic.Ext.applyExtTheorem
+:::
+
+:::tactic "funext"
+:::
+
+# Simplification
+
+The simplifier is described in greater detail in {ref "the-simplifier"}[its dedicated chapter].
+
+:::tactic "simp"
+:::
+
+:::tactic "simp!"
+:::
+
+:::tactic "simp?"
+:::
+
+:::tactic "simp?!"
+:::
+
+:::tactic "simp_arith"
+:::
+
+:::tactic "simp_arith!"
+:::
+
+:::tactic "dsimp"
+:::
+
+:::tactic "dsimp!"
+:::
+
+:::tactic "dsimp?"
+:::
+
+:::tactic "dsimp?!"
+:::
+
+
+:::tactic "simp_all"
+:::
+
+:::tactic "simp_all!"
+:::
+
+:::tactic "simp_all?"
+:::
+
+:::tactic "simp_all?!"
+:::
+
+
+:::tactic "simp_all_arith"
+:::
+
+
+:::tactic "simp_all_arith!"
+:::
+
+
+:::tactic "simpa"
+:::
+
+
+:::tactic "simpa!"
+:::
+
+:::tactic "simpa?"
+:::
+
+:::tactic "simpa?!"
+:::
+
+:::tactic "simp_wf"
+:::
+
+# Rewriting
+
+:::tactic "rw"
+:::
+
+:::tactic "rewrite"
+:::
+
+:::tactic "erw"
+:::
+
+:::tactic Lean.Parser.Tactic.tacticRwa__
+:::
+
+:::tactic "unfold"
+
+Implemented by {name}`Lean.Elab.Tactic.evalUnfold`.
+:::
+
+:::tactic "replace"
+:::
+
+:::tactic "delta"
+:::
+
+
+# Inductive Types
+
+## Introduction
+
+:::tactic "constructor"
+:::
+
+
+:::tactic "injection"
+:::
+
+:::tactic "injections"
+:::
+
+:::tactic "left"
+:::
+
+:::tactic "right"
+:::
+
+## Elimination
+
+:::planned
+
+Description of the `@[induction_eliminator]` and `@[cases_eliminator]` attributes
+
+:::
+
+:::tactic "cases"
+:::
+
+:::tactic "rcases"
+:::
+
+:::tactic "induction"
+:::
+
+:::tactic "nofun"
+:::
+
+:::tactic "nomatch"
+:::
+
+
+# Library Search
+
+The library search tactics are intended for interactive use.
+When run, they search the Lean library for lemmas or rewrite rules that could be applicable in the current situation, and suggests a new tactic.
+These tactics should not be left in a proof; rather, their suggestions should be incorporated.
+
+:::tactic "exact?"
+:::
+
+:::tactic "apply?"
+:::
+
+
+
+
+:::tacticExample
+{goal show:=false}`∀ (i j k : Nat), i < j → j < k → i < k`
+```setup
+intro i j k h1 h2
+```
+In this proof state:
+```pre
+i j k : Nat
+h1 : i < j
+h2 : j < k
+⊢ i < k
+```
+
+invoking {tacticStep}`apply?` suggests:
+
+```tacticOutput
+Try this: exact Nat.lt_trans h1 h2
+```
+
+```post (show := false)
+
+```
+:::
+
+
+:::tactic "rw?"
+:::
+
+# Case Analysis
+
+:::tactic "split"
+:::
+
+:::tactic "by_cases"
+:::
+
+# Decision Procedures
+
+:::tactic Lean.Parser.Tactic.decide show:="decide"
+:::
+
+:::tactic Lean.Parser.Tactic.nativeDecide show:="native_decide"
+:::
+
+:::tactic "omega"
+:::
+
+:::tactic "bv_omega"
+:::
+
+
+## SAT Solver Integration
+
+
+:::tactic "bv_decide"
+:::
+
+:::tactic "bv_normalize"
+:::
+
+:::tactic "bv_check"
+:::
+
+:::tactic Lean.Parser.Tactic.bvTrace
+:::
+
+# Control Flow
+
+:::tactic "skip"
+:::
+
+
+:::tactic Lean.Parser.Tactic.guardHyp
+:::
+
+:::tactic Lean.Parser.Tactic.guardTarget
+:::
+
+:::tactic Lean.Parser.Tactic.guardExpr
+:::
+
+:::tactic "done"
+:::
+
+:::tactic "sleep"
+:::
+
+
+:::tactic "checkpoint"
+:::
+
+:::tactic "save"
+:::
+
+:::tactic "stop"
+:::
+
+
+# Term Elaboration Backends
+
+These tactics are used during elaboration of terms to satisfy obligations that arise.
+
+:::tactic "decreasing_tactic"
+:::
+
+:::tactic "decreasing_trivial"
+:::
+
+:::tactic "array_get_dec"
+:::
+
+:::tactic tacticDecreasing_with_
+:::
+
+
+:::tactic "get_elem_tactic"
+:::
+
+:::tactic "get_elem_tactic_trivial"
+:::
+
+
+
+# Debugging Utilities
+
+:::tactic "sorry"
+:::
+
+:::tactic "admit"
+:::
+
+:::tactic "dbg_trace"
+:::
+
+:::tactic Lean.Parser.Tactic.traceState
+:::
+
+:::tactic Lean.Parser.Tactic.traceMessage
+:::
+
+
+# Other
+
+:::tactic "trivial"
+:::
+
+:::tactic "solve"
+:::
+
+:::tactic "and_intros"
+:::
+
+:::tactic "infer_instance"
+:::
+
+:::tactic Lean.Parser.Tactic.tacticUnhygienic_
+:::
+
+:::tactic Lean.Parser.Tactic.runTac
+:::
