Manual/Terms.lean
@@ -1,0 +1,24 @@
+import VersoManual
+
+import Manual.Meta
+
+open Verso.Genre Manual
+
+set_option pp.rawOnError true
+
+set_option linter.unusedVariables false
+
+#doc (Manual) "Terms" =>
+
+::: planned
+This chapter will describe Lean's term language, including the following features:
+ * Name resolution, including variable occurrences, `open` declarations and terms
+ * Function application, including implicit, instance, and named arguments
+ * Leading `.`-notation and accessor notation
+ * `fun`, with and without pattern matching
+ * Literals (some via cross-references to the appropriate types, e.g. {name}`String`)
+ * Conditionals and their relationship to {name}`Decidable`
+ * Pattern matching, including `match`, `let`, `if let`, `matches`, `nomatch`, `nofun`
+ * Do-notation, including `let mut`, `for`, `while`, `repeat`, `break`, `return`
+ * {deftech}_Holes_ and {deftech}_named holes_
+:::
